platform/RelDbSelect.v
@@ -1,0 +1,589 @@
+Require Import AutoSep Wrap StringOps Malloc ArrayOps Buffers Bags.
+Require Import SinglyLinkedList ListSegment RelDb.
+
+Set Implicit Arguments.
+
+
+(** * Iterating over matching rows of a table *)
+
+Opaque mult.
+Local Infix ";;" := SimpleSeq : SP_scope.
+
+Section Select.
+  Variable A : Type.
+  Variable invPre : A -> vals -> HProp.
+  Variable invPost : A -> vals -> W -> HProp.
+
+  Variable tptr : W.
+  Variable sch : schema.
+
+  (* Store a pointer to the current linked list node and actual row data, respectively,
+   * in these variables. *)
+  Variables rw data : string.
+
+  (* Test to use in filtering rows *)
+  Variable cond : condition.
+
+  (* Run this command on every matching row. *)
+  Variable body : (W -> W -> HProp) -> chunk.
+  (* The argument to [body] is an invariant to preserve.
+   * Its inputs are the values of [rw] and [data]. *)
+
+  Section compileEquality.
+    (* One field test, storing Boolean result in "matched" *)
+    Definition compileEquality (e : equality) : chunk :=
+      match resolve sch (fst e) with
+        | None => Fail
+        | Some offset =>
+          "tmp" <- data;;
+          "ibuf" <-* "tmp";;
+          "ilen" <-* "tmp" + 4;;
+
+          Assert [Al bs, Al a : A, Al head, Al done, Al remaining, Al rcols, Al rbs,
+            PRE[V] array8 bs (V "buf") * [| length bs = wordToNat (V "len") |]
+              * [| inputOk V (exps cond) |]
+              * [| V rw <> 0 |] * tptr =*> head * lseg done head (V rw) * sll (V data :: remaining) (V rw)
+              * rows sch head remaining * rows sch head done * invPre a V
+              * (V data ==*> V "ibuf", V "ilen") * array (posl rcols) (V data ^+ $8)
+              * array (lenl rcols) (V data ^+ $8 ^+ $(length sch * 4)) * array8 rbs (V "ibuf")
+              * [| length rbs = wordToNat (V "ilen") |] * [| length rcols = length sch |]
+              * [| inBounds (V "ilen") rcols |] * [| V data <> 0 |]
+              * [| freeable (V data) (2 + length sch + length sch) |]
+              * [| V "ibuf" <> 0 |] * [| freeable8 (V "ibuf") (length rbs) |]
+              * [| natToW offset < natToW (length (posl rcols)) |]%word
+            POST[R] array8 bs (V "buf") * invPost a V R];;
+
+          "tmp" <- data + 8;;
+          "ipos" <-* "tmp" + (4 * offset)%nat;;
+
+          Assert [Al bs, Al a : A, Al head, Al done, Al remaining, Al rcols, Al rbs,
+            PRE[V] array8 bs (V "buf") * [| length bs = wordToNat (V "len") |]
+              * [| inputOk V (exps cond) |]
+              * [| V rw <> 0 |] * tptr =*> head * lseg done head (V rw) * sll (V data :: remaining) (V rw)
+              * rows sch head remaining * rows sch head done * invPre a V
+              * (V data ==*> V "ibuf", V "ilen") * array (posl rcols) (V data ^+ $8)
+              * array (lenl rcols) (V data ^+ $8 ^+ $(length sch * 4)) * array8 rbs (V "ibuf")
+              * [| length rbs = wordToNat (V "ilen") |] * [| length rcols = length sch |]
+              * [| inBounds (V "ilen") rcols |] * [| V data <> 0 |]
+              * [| freeable (V data) (2 + length sch + length sch) |]
+              * [| V "ibuf" <> 0 |] * [| freeable8 (V "ibuf") (length rbs) |]
+              * [| V "ipos" = Array.selN (posl rcols) offset |]
+              * [| natToW offset < natToW (length (lenl rcols)) |]%word
+            POST[R] array8 bs (V "buf") * invPost a V R];;
+
+          "tmp" <- data + 8;;
+          "tmp" <- "tmp" + (length sch * 4)%nat;;
+          "tmp" <-* "tmp" + (4 * offset)%nat;;
+
+          Assert [Al bs, Al a : A, Al head, Al done, Al remaining, Al rcols, Al rbs,
+            PRE[V] array8 bs (V "buf") * [| length bs = wordToNat (V "len") |]
+              * [| inputOk V (exps cond) |]
+              * [| V rw <> 0 |] * tptr =*> head * lseg done head (V rw) * sll (V data :: remaining) (V rw)
+              * rows sch head remaining * rows sch head done * invPre a V
+              * (V data ==*> V "ibuf", V "ilen") * array (posl rcols) (V data ^+ $8)
+              * array (lenl rcols) (V data ^+ $8 ^+ $(length sch * 4)) * array8 rbs (V "ibuf")
+              * [| length rbs = wordToNat (V "ilen") |] * [| length rcols = length sch |]
+              * [| inBounds (V "ilen") rcols |] * [| V data <> 0 |]
+              * [| freeable (V data) (2 + length sch + length sch) |]
+              * [| V "ibuf" <> 0 |] * [| freeable8 (V "ibuf") (length rbs) |]
+              * [| V "ipos" = Array.selN (posl rcols) offset |]
+              * [| V "tmp" = Array.selN (lenl rcols) offset |]
+            POST[R] array8 bs (V "buf") * invPost a V R];;
+
+          match snd e with
+            | Const s =>
+              If ("tmp" <> String.length s) {
+                (* Field value has wrong length to match. *)
+                "matched" <- 0
+              } else {
+                StringEq "ibuf" "ilen" "ipos" "matched" s
+                (fun (a_bs : A * list B) V => array8 (snd a_bs) (V "buf")
+                  * [| length (snd a_bs) = wordToNat (V "len") |]
+                  * [| inputOk V (exps cond) |]
+                  * Ex head, Ex done, Ex remaining, Ex rcols,
+                    [| V rw <> 0 |] * tptr =*> head * lseg done head (V rw)
+                    * sll (V data :: remaining) (V rw)
+                    * rows sch head remaining * rows sch head done
+                    * invPre (fst a_bs) V
+                    * (V data ==*> V "ibuf", V "ilen") * array (posl rcols) (V data ^+ $8)
+                    * array (lenl rcols) (V data ^+ $8 ^+ $(length sch * 4))
+                    * [| length rcols = length sch |]
+                    * [| inBounds (V "ilen") rcols |] * [| V data <> 0 |]
+                    * [| freeable (V data) (2 + length sch + length sch) |]
+                    * [| V "ibuf" <> 0 |] * [| freeable8 (V "ibuf") (wordToNat (V "ilen")) |]
+                    * [| V "ipos" = Array.selN (posl rcols) offset |])%Sep
+                (fun _ a_bs V R => array8 (snd a_bs) (V "buf") * invPost (fst a_bs) V R)%Sep
+              }
+            | Input pos len =>
+              If ("tmp" <> len) {
+                "matched" <- 0
+              } else {
+                "matched" <-- Call "array8"!"equal"("ibuf", "ipos", "buf", pos, len)
+                [Al bs, Al a : A, Al head, Al done, Al remaining,
+                  PRE[V] array8 bs (V "buf") * [| length bs = wordToNat (V "len") |]
+                    * [| inputOk V (exps cond) |]
+                    * [| V rw <> 0 |] * tptr =*> head * lseg done head (V rw)
+                    * sll (V data :: remaining) (V rw)
+                    * rows sch head remaining * rows sch head done * row sch (V data) * invPre a V
+                  POST[R] array8 bs (V "buf") * invPost a V R]
+              }
+          end
+      end%SP.
+
+    Variable mn : string.
+    Variable im : LabelMap.t assert.
+    Variable H : importsGlobal im.
+    Variable ns : list string.
+    Variable res : nat.
+
+    Definition eqinv' := Al bs, Al a : A, Al head, Al done, Al remaining,
+      PRE[V] array8 bs (V "buf") * [| length bs = wordToNat (V "len") |]
+        * [| inputOk V (exps cond) |]
+        * [| V rw <> 0 |] * tptr =*> head * lseg done head (V rw) * sll (V data :: remaining) (V rw)
+        * rows sch head remaining * rows sch head done * row sch (V data) * invPre a V
+      POST[R] array8 bs (V "buf") * invPost a V R.
+
+    Definition eqinv := eqinv' true (fun w => w).
+
+    Hypothesis not_rp : ~In "rp" ns.
+    Hypothesis included : incl baseVars ns.
+    Hypothesis reserved : (res >= 10)%nat.
+    Hypothesis wellFormed : wfEqualities ns sch cond.
+
+    Hypothesis weakenPre : (forall a V V', (forall x, x <> "ibuf" -> x <> "row" -> x <> "ilen" -> x <> "tmp"
+      -> x <> "ipos" -> x <> "overflowed" -> x <> "matched" -> sel V x = sel V' x)
+    -> invPre a V ===> invPre a V').
+
+    Hypothesis weakenPost : (forall a V V' R, (forall x, x <> "ibuf" -> x <> "row" -> x <> "ilen" -> x <> "tmp"
+      -> x <> "ipos" -> x <> "overflowed" -> x <> "matched" -> sel V x = sel V' x)
+    -> invPost a V R = invPost a V' R).
+
+    Lemma resolve_ok : forall e s,
+      wfEquality ns s e
+      -> exists offset, resolve s (fst e) = Some offset
+        /\ (offset < length s)%nat.
+      unfold wfEquality; induction s; simpl; intuition subst;
+        match goal with
+          | [ |- context[if ?E then _ else _] ] => destruct E
+        end; intuition eauto.
+      destruct H1; intuition idtac.
+      rewrite H3; eauto.
+    Qed.
+
+    Hypothesis matched_rw : "matched" <> rw.
+    Hypothesis matched_data : "matched" <> data.
+
+    Lemma compileEquality_post : forall e pre,
+      wfEquality ns sch e
+      -> (forall specs st,
+        interp specs (pre st)
+        -> interp specs (eqinv ns res st))
+      -> forall specs st,
+        interp specs (Postcondition (toCmd (compileEquality e) mn (im := im) H ns res pre) st)
+        -> interp specs (eqinv ns res st).
+      unfold compileEquality; intros.
+      match goal with
+        | [ H : _ |- _ ] => destruct (resolve_ok H); intuition idtac; destruct H
+      end.
+      match goal with
+        | [ H : resolve _ _ = _ |- _ ] => rewrite H in *
+      end.
+      destruct e as [ ? [ ] ]; simpl in *; intuition idtac.
+
+      v.
+      v.
+    Qed.
+
+    Hypothesis equal : "array8"!"equal" ~~ im ~~> ArrayOps.equalS.
+
+    Hypothesis data_rp : data <> "rp".
+    Hypothesis data_ibuf : data <> "ibuf".
+    Hypothesis data_ipos : data <> "ipos".
+    Hypothesis data_ilen : data <> "ilen".
+    Hypothesis data_tmp : data <> "tmp".
+    Hypothesis data_ns : In data ns.
+
+    Hypothesis rw_rp : rw <> "rp".
+    Hypothesis rw_ibuf : rw <> "ibuf".
+    Hypothesis rw_ipos : rw <> "ipos".
+    Hypothesis rw_ilen : rw <> "ilen".
+    Hypothesis rw_tmp : rw <> "tmp".
+
+    Hypothesis goodSize_sch : goodSize (length sch).
+
+    Lemma length_posl : forall ls, length (posl ls) = length ls.
+      clear; induction ls; simpl; intuition.
+    Qed.
+
+    Lemma length_lenl : forall ls, length (lenl ls) = length ls.
+      clear; induction ls; simpl; intuition.
+    Qed.
+
+    Lemma length_match : forall x (ls : list (W * W)),
+      (x < length sch)%nat
+      -> length ls = length sch
+      -> natToW x < natToW (Datatypes.length ls).
+      generalize goodSize_sch; clear; intros.
+      pre_nomega.
+      rewrite wordToNat_natToWord_idempotent.
+      rewrite wordToNat_natToWord_idempotent.
+      congruence.
+      rewrite H0; assumption.
+      change (goodSize x); eapply goodSize_weaken; eauto.
+    Qed.
+
+    Lemma length_match_posl : forall x ls,
+      (x < length sch)%nat
+      -> length ls = length sch
+      -> natToW x < natToW (Datatypes.length (posl ls)).
+      intros; rewrite length_posl; auto using length_match.
+    Qed.
+
+    Lemma length_match_lenl : forall x ls,
+      (x < length sch)%nat
+      -> length ls = length sch
+      -> natToW x < natToW (Datatypes.length (lenl ls)).
+      intros; rewrite length_lenl; auto using length_match.
+    Qed.
+
+    Hint Immediate length_match_posl length_match_lenl.
+
+    Lemma selN_col : forall x ls,
+      (x < length sch)%nat
+      -> Array.sel ls (natToW x) = selN ls x.
+      generalize goodSize_sch; clear; unfold Array.sel; intros; f_equal.
+      apply wordToNat_natToWord_idempotent.
+      change (goodSize x).
+      eapply goodSize_weaken; eauto.
+    Qed.
+
+    Hint Immediate selN_col.
+
+    Lemma inBounds_selN' : forall len cols,
+      inBounds len cols
+      -> forall col, (col < length cols)%nat
+        -> (wordToNat (selN (posl cols) col) + wordToNat (selN (lenl cols) col) <= wordToNat len)%nat.
+      clear; induction cols; inversion 1; simpl; intuition; destruct col; intuition.
+    Qed.
+
+    Lemma inBounds_selN : forall len cols,
+      inBounds len cols
+      -> forall col a b c, a = selN (posl cols) col
+        -> b = selN (lenl cols) col
+        -> c = wordToNat len
+        -> (col < length cols)%nat
+        -> (wordToNat a + wordToNat b <= c)%nat.
+      intros; subst; eauto using inBounds_selN'.
+    Qed.
+
+    Hint Extern 1 (_ + _ <= _)%nat =>
+      eapply inBounds_selN; try eassumption; (cbv beta; congruence).
+
+    Lemma weakened_bound : forall pos cols x len,
+      inBounds len cols
+      -> pos = selN (posl cols) x
+      -> (x < length cols)%nat
+      -> pos <= len.
+      clear; intros; subst.
+      eapply inBounds_selN in H; try (reflexivity || eassumption).
+      nomega.
+    Qed.
+
+    Hint Extern 1 (_ <= _) => eapply weakened_bound; try eassumption; (cbv beta; congruence).
+
+    Hint Resolve use_inputOk.
+
+    Lemma In_exps : forall s e c,
+      In (s, e) c
+      -> In e (exps c).
+      clear; induction c; simpl; intuition (subst; auto).
+    Qed.
+
+    Hint Immediate In_exps.
+
+    Lemma compileEquality_vcs : forall e pre,
+      wfEquality ns sch e
+      -> In e cond
+      -> (forall specs st,
+        interp specs (pre st)
+        -> interp specs (eqinv ns res st))
+      -> vcs (VerifCond (toCmd (compileEquality e) mn (im := im) H ns res pre)).
+        unfold compileEquality; intros.
+        match goal with
+          | [ H : _ |- _ ] => destruct (resolve_ok H); intuition idtac; destruct H
+        end.
+        match goal with
+          | [ H : resolve _ _ = _ |- _ ] => rewrite H in *
+        end.
+        wrap0.
+
+        v.
+        v.
+        v.
+        v.
+        v.
+        v.
+        v.
+        v.
+        v.
+        v.
+        v.
+
+        destruct e as [ ? [ ] ]; simpl in *; intuition idtac.
+        
+        repeat match goal with
+                 | [ |- vcs _ ] => constructor
+               end; intros.
+
+        v.
+        v.
+        v.
+        v.
+        v.
+        v.
+        v.
+        v.
+        v.
+        v.
+        v.
+        v.
+        v.
+        v.
+        v.
+        v.
+        v.
+
+        repeat match goal with
+                 | [ |- vcs _ ] => constructor
+               end; intros.
+
+        (* Something bizarre is happening here, with [destruct] not clearing a hypothesis
+         * within [propxFo]. *)
+        apply simplify_fwd in H25.
+        repeat match goal with
+                 | [ H : simplify _ (Ex x, _) _ |- _ ] => destruct H
+               end.
+        apply simplify_bwd in H25.
+        v.
+
+        v.
+        v.
+        v.
+        v.
+      Qed.
+
+    Fixpoint compileEqualities (es : condition) : chunk :=
+      match es with
+        | nil => "matched" <- 1
+        | e :: es' =>
+          compileEquality e;;
+          If ("matched" = 0) {
+            Skip
+          } else {
+            compileEqualities es'
+          }
+      end%SP.
+
+    Lemma wfEqualities_inv1 : forall ns sch e es,
+      wfEqualities ns sch (e :: es)
+      -> wfEquality ns sch e.
+      inversion 1; auto.
+    Qed.
+
+    Lemma wfEqualities_inv2 : forall ns sch e es,
+      wfEqualities ns sch (e :: es)
+      -> wfEqualities ns sch es.
+      inversion 1; auto.
+    Qed.
+
+    Hint Immediate wfEqualities_inv1 wfEqualities_inv2.
+
+    Lemma compileEqualities_post : forall es pre,
+      wfEqualities ns sch es
+      -> (forall specs st,
+        interp specs (pre st)
+        -> interp specs (eqinv ns res st))
+      -> forall specs st,
+        interp specs (Postcondition (toCmd (compileEqualities es) mn (im := im) H ns res pre) st)
+        -> interp specs (eqinv ns res st).
+      induction es; simpl; intuition idtac;
+        (pre;
+          repeat (match goal with
+                    | [ H : interp _ (Postcondition (toCmd (compileEquality _) _ _ _ _ _) _) |- _ ] =>
+                      apply compileEquality_post in H
+                    | [ IH : forall pre : _ -> _, _, H : interp _ (Postcondition _ _) |- _ ] =>
+                      apply IH in H
+                  end; eauto; pre); t).
+    Qed.
+
+    Lemma compileEqualities_vcs : forall es pre,
+      wfEqualities ns sch es
+      -> incl es cond
+      -> (forall specs st,
+        interp specs (pre st)
+        -> interp specs (eqinv ns res st))
+      -> vcs (VerifCond (toCmd (compileEqualities es) mn (im := im) H ns res pre)).
+      induction es; intros; try match goal with
+                                  | [ H : incl _ cond |- _ ] => apply incl_peel in H
+                                end; wrap0;
+      (repeat (match goal with
+                 | _ => apply compileEquality_vcs
+                 | [ H : interp _ (Postcondition (toCmd (compileEquality _) _ _ _ _ _) _) |- _ ] =>
+                   apply compileEquality_post in H
+                 | [ IH : forall pre : _ -> _, _ |- vcs _ ] =>
+                   apply IH
+               end; eauto; pre); t).
+    Qed.
+  End compileEquality.
+
+  Definition Select' : chunk := (
+    rw <-* tptr;;
+
+    [Al bs, Al a : A, Al head, Al done, Al remaining,
+      PRE[V] array8 bs (V "buf") * [| length bs = wordToNat (V "len") |] * [| inputOk V (exps cond) |]
+        * tptr =*> head * lseg done head (V rw) * sll remaining (V rw)
+        * rows sch head done * rows sch head remaining * invPre a V
+      POST[R] array8 bs (V "buf") * invPost a V R]
+    While (rw <> 0) {
+      data <-* rw;;
+
+      Assert [Al bs, Al a : A, Al head, Al done, Al remaining,
+        PRE[V] array8 bs (V "buf") * [| length bs = wordToNat (V "len") |] * [| inputOk V (exps cond) |]
+          * [| V rw <> 0 |] * tptr =*> head * lseg done head (V rw) * sll (V data :: remaining) (V rw)
+          * rows sch head remaining * rows sch head done * row sch (V data) * invPre a V
+        POST[R] array8 bs (V "buf") * invPost a V R];;
+
+      compileEqualities cond;;
+
+      If ("matched" = 0) {
+        Skip
+      } else {
+        body (fun V_rw V_data => Ex head, Ex done, Ex remaining, Ex p,
+          tptr =*> head * lseg done head V_rw
+          * (V_rw ==*> V_data, p) * sll remaining p
+          * rows sch head done * rows sch head remaining
+          * [| freeable V_rw 2 |] * [| V_rw <> 0 |])%Sep
+      };;
+
+      rw <-* rw + 4;;
+
+      Assert [Al bs, Al a : A, Al head, Al done, Al remaining,
+        PRE[V] array8 bs (V "buf") * [| length bs = wordToNat (V "len") |] * [| inputOk V (exps cond) |]
+          * tptr =*> head * lseg_append (done ++ V data :: nil) head (V rw) * sll remaining (V rw)
+          * rows sch head (done ++ V data :: nil) * rows sch head remaining * invPre a V
+        POST[R] array8 bs (V "buf") * invPost a V R]
+    }
+  )%SP.
+
+  Definition sinvar :=
+    Al bs, Al a : A,
+    PRE[V] array8 bs (V "buf") * [| length bs = wordToNat (V "len") |] * [| inputOk V (exps cond) |]
+      * table sch tptr * invPre a V
+    POST[R] array8 bs (V "buf") * invPost a V R.
+
+  Definition spost inv :=
+    Al bs, Al a : A,
+    PRE[V] array8 bs (V "buf") * [| length bs = wordToNat (V "len") |] * [| inputOk V (exps cond) |]
+      * row sch (V data) * inv (V rw) (V data) * invPre a V
+    POST[R] array8 bs (V "buf") * invPost a V R.
+
+  Notation svars := (rw :: data :: nil).
+
+  Definition noOverlapExp (e : exp) :=
+    match e with
+      | Const _ => True
+      | Input pos len => pos <> rw /\ pos <> data /\ len <> rw /\ len <> data
+    end.
+
+  Definition noOverlapExps := List.Forall noOverlapExp.
+
+  Notation SelectVcs := (fun im ns res =>
+    (~In "rp" ns) :: incl svars ns :: (rw <> "rp")%type :: (data <> "rp")%type
+    :: incl baseVars ns
+    :: (rw <> data)%type
+    :: (forall a V V', (forall x, x <> rw -> x <> data
+      -> x <> "ibuf" -> x <> "row" -> x <> "ilen" -> x <> "tmp"
+      -> x <> "ipos" -> x <> "overflowed" -> x <> "matched" -> sel V x = sel V' x)
+      -> invPre a V ===> invPre a V')
+    :: (forall a V V' R, (forall x, x <> rw -> x <> data
+      -> x <> "ibuf" -> x <> "row" -> x <> "ilen" -> x <> "tmp"
+      -> x <> "ipos" -> x <> "overflowed" -> x <> "matched" -> sel V x = sel V' x)
+      -> invPost a V R = invPost a V' R)
+    :: (forall inv pre mn H,
+      (forall specs st, interp specs (pre st)
+        -> interp specs (spost inv true (fun w => w) ns res st))
+      -> vcs (VerifCond (toCmd (body inv) mn (im := im) H ns res pre)))
+    :: (forall specs inv pre mn H st,
+      interp specs (Postcondition (toCmd (body inv) mn (im := im) H ns res pre) st)
+      -> interp specs (spost inv true (fun w => w) ns res st))
+    :: "array8"!"equal" ~~ im ~~> ArrayOps.equalS
+    :: (res >= 10)%nat
+    :: wfEqualities ns sch cond
+    :: ("matched" <> rw)%type
+    :: ("matched" <> data)%type
+    :: (data <> "ibuf")%type
+    :: (data <> "ipos")%type
+    :: (data <> "ilen")%type
+    :: (data <> "tmp")%type
+    :: (data <> "len")%type
+    :: (data <> "buf")%type
+    :: In data ns
+    :: (rw <> "rp")%type
+    :: (rw <> "ibuf")%type
+    :: (rw <> "ipos")%type
+    :: (rw <> "ilen")%type
+    :: (rw <> "tmp")%type
+    :: (rw <> "len")%type
+    :: (rw <> "buf")%type
+    :: goodSize (length sch)
+    :: noOverlapExps (exps cond)
+    :: nil).
+
+  Hint Immediate incl_refl.
+
+  Theorem Forall_impl3 : forall A (P Q R S : A -> Prop) ls,
+    List.Forall P ls
+    -> List.Forall Q ls
+    -> List.Forall R ls
+    -> (forall x : A, P x -> Q x -> R x -> S x)
+    -> List.Forall S ls.
+    induction 1; inversion 1; inversion 1; auto.
+  Qed.
+
+  Theorem inputOk_weaken_params : forall ns V V' es,
+    inputOk V es
+    -> noOverlapExps es
+    -> wfExps ns es
+    -> (forall x, x <> rw -> x <> data -> sel V x = sel V' x)
+    -> rw <> "len"
+    -> data <> "len"
+    -> inputOk V' es.
+    intros; eapply Forall_impl3; [ apply H | apply H0 | apply H1 | ].
+    intro e; destruct e; simpl; intuition idtac.
+    repeat rewrite <- H2 by (simpl; congruence); assumption.
+  Qed.
+
+  Hint Extern 2 (inputOk _ _) => eapply inputOk_weaken_params; try eassumption;
+    try (eapply wfEqualities_wfExps; eassumption); [ descend ].
+
+  Hint Resolve compileEqualities_vcs.
+
+  Ltac q :=
+    repeat match goal with
+             | [ H : interp _ _, _ : context[Binop _ _ Plus (immInR (natToW 4) _)] |- _ ] =>
+               apply compileEqualities_post in H; auto; pre; prep; evalu;
+                 match goal with
+                   | [ _ : _ = _ :: ?ls |- _ ] => do 4 eexists; exists ls
+                 end
+             | [ H : interp _ _ |- _ ] => apply compileEqualities_post in H; auto
+             | [ H : _ |- vcs _ ] => apply H; pre
+           end; t.
+
+  Definition Select : chunk.
+    refine (WrapC Select'
+      sinvar
+      sinvar
+      SelectVcs
+      _ _); abstract (wrap0; abstract q).
+  Qed.
+End Select.
